Progress on Spec.AES128_CBC

specs/Spec.AES128_CBC.fst
@@ -31,19 +31,44 @@ let cbc_decrypt_block iv key block =
   map2 (^.) iv aes_output
 
 
-val cbc_encrypt_last: iv -> key -> input:bytes{length input < size_block} -> Tot block
+val cbc_encrypt_last: iv -> key -> input:bytes{length input < size_block} -> FStar.All.ML block
 let cbc_encrypt_last iv key input =
   let len = length input in
   let block = create size_block (u8 (size_block - len)) in
   let block = update_sub block 0 len input in
-  cbc_encrypt_block iv key block
+  let res = cbc_encrypt_block iv key block in
+  IO.print_string "\nencrypt_last (block): \n";
+  List.iter (fun a -> IO.print_uint8 (u8_to_UInt8 a);  IO.print_string ":") (to_list block);
+  IO.print_string "\n";
+  res
+
+
+val unpadPKCS: block -> idx:size_nat{idx < size_block} -> Tot (option bytes)
+let rec unpadPKCS b idx =
+  let last_byte = b.[size_block - 1] in
+  let vpad = uint_v last_byte in
+  if vpad <= size_block then
+    if (size_block - vpad) < idx then (
+      if uint_v b.[idx] = uint_v last_byte then unpadPKCS b (idx - 1) else None)
+    else (
+      let plaintext = sub #uint8 #size_block b 0 (size_block - vpad) in
+      Some plaintext)
+  else None
+
+val cbc_decrypt_last: iv -> key -> block -> FStar.All.ML (option bytes)
+let cbc_decrypt_last iv k b =
+  let plain_block = cbc_decrypt_block iv k b in
+  IO.print_string "\ndecrypt_last (block): \n";
+  List.iter (fun a -> IO.print_uint8 (u8_to_UInt8 a);  IO.print_string ":") (to_list plain_block);
+  IO.print_string "\n";
+  unpadPKCS plain_block (size_block - 1)
 
 
 val aes128_cbc_encrypt:
-    input: bytes{length input * size_block <= max_size_t}
+    input: bytes{length input + size_block <= max_size_t}
   -> k: key
   -> iv: iv ->
-  Tot (ciphertext:bytes)
+  FStar.All.ML (ciphertext:bytes)
 
 let aes128_cbc_encrypt input k iv =
   let len = length input in
@@ -55,26 +80,34 @@ let aes128_cbc_encrypt input k iv =
     cipher_block, cipher_block) iv in
   if rem <> 0 then (
     let last = sub #uint8 #len input (n * size_block) rem in
-    ciphertext @| (cbc_encrypt_last last_iv k last))
+    let last_cipher_block = cbc_encrypt_last last_iv k last in
+    ciphertext @| last_cipher_block)
   else (
     let padding = create size_block (u8 size_block) in
     let last_cipher_block = cbc_encrypt_block last_iv k padding in
     ciphertext @| last_cipher_block)
 
 
-(* val aes128_cbc_decrypt: *)
-(*     input: bytes{length input % size_block == 0} *)
-(*   -> k: key *)
-(*   -> iv: iv -> *)
-(*   Tot (option bytes) *)
+val aes128_cbc_decrypt:
+    input: bytes{size_block <= length input
+               /\ length input % size_block == 0
+               /\ length input <= max_size_t}
+  -> k: key
+  -> iv: iv ->
+  FStar.All.ML (option bytes)
 
-(* let aes128_cbc_decrypt ciphertext k iv = *)
-(*   let clen = length ciphertext in *)
-(*   let n = clen / size_block in *)
-(*   let _, plaintext = generate_blocks size_block n (fun _ -> block) (fun i iv -> *)
-(*     let cblock_i = sub #uint8 #clen ciphertext (i * size_block) size_block in *)
-(*     let plain_block = cbc_decrypt_block iv k cblock_i in *)
-(*     cblock_i, plain_block) iv in *)
-(*   let last_byte = plaintext.[clen - 1] in *)
-(*   if last_byte > size_block then None *)
-(*   else if plaintext.[clen - las] *)
+let aes128_cbc_decrypt ciphertext k iv =
+  let clen : size_nat = length ciphertext in
+  let n : size_nat = clen / size_block in
+  let last_iv, plaintext = generate_blocks size_block (n - 1) (fun _ -> block) (fun i iv ->
+    let cblock_i = sub #uint8 #clen ciphertext (i * size_block) size_block in
+    let plain_block = cbc_decrypt_block iv k cblock_i in
+    cblock_i, plain_block) iv in
+  IO.print_string "\nComputed plaintext (blocks): \n";
+  List.iter (fun a -> IO.print_uint8 (u8_to_UInt8 a);  IO.print_string ":") (to_list plaintext);
+  IO.print_string "\n";
+let last_cipher_block = sub #uint8 #clen ciphertext ((n - 1) * size_block) size_block in
+  match cbc_decrypt_last last_iv k last_cipher_block with
+  | None -> None
+  | Some last_plain_block ->
+    Some (Seq.Base.append plaintext last_plain_block)
